\documentclass[12pt,letterpaper,final]{report}

\begin{document}


\fbox{
\vbox{
\begin{flushleft}
Name \\  % authors' names
COSC 336 \\  %class
08/29/2024\\  % date
\end{flushleft}
\center{\Large{\textbf{Assignment 3 Exercise 1.}}}
%\end{mdframed}
} % end vbox
} % end fbox
\vline

\noindent\textbf{Exercise 1.}  

\textbf{}

For each of the following functions, give a $\Theta(t(n))$ estimation with the simplest possible $t(n)$ (for example $3n^2 +5 n \log n = \Theta(n^2)$).

\begin{enumerate}

\item $13n^2 - 2n + 56$
\newline $t(n) = \Theta(n^2)$

\item $2.5 \log n + 2$
\newline $t(n) = \Theta(\log n)$

\item $n (12 + \log n)$
\newline $n (12 + \log n) = 12n + n \log n$
\newline $t(n) = \Theta(n \log n)$


\item $1+2 + 3 + \ldots + 2n$
\newline
\newline $S_n = \frac{n(n + 1)}{2}$
\newline $S_{2n} = \frac{2n(2n + 1)}{2}$
\newline $\frac{2n(2n + 1)}{2} = n (2n +1) = {2n^2} + n$
\newline $t(n) = \Theta(n^{2})$

\item $1+2 + 3 + \ldots + n^2$
\newline
\newline $S_n = \frac{n(n + 1)}{2}$
\newline $S_{n^2} = \frac{n^2(n^2 + 1)}{2}$
\newline $\frac{n^2(n^2 + 1)}{2} = \frac{n^4 + n^2}{2}$
\newline $t(n) = \Theta(n^{4})$

\item $\log (n^3) + 10$
\newline $\log (n^3) = 3\log n $
\newline $t(n) = \Theta(\log n)$

\item $\log(n^3) + n \log n$
\newline $ \log (n^3) = 3 \log n $
\newline $t(n) = \Theta(n \log n)$

\item $n \log (n^3) + n \log n$
\newline $ n \log (n^3) = 3n \log n $
\newline $t(n) = \Theta(n \log n)$

\item $2^{2 \log n} + 5n +1$
\newline $2^{2 \log n} = (2^{\log n})^2 = n^2$
\newline $t(n) = \Theta(n^{2})$

\end{enumerate}
\bigskip


\end{document}